Don't include the global environment in semantics
Global environments are used as intermediate constructions when defining
the step relation for individual languages, however there is no need to
include them in the common interface for small-step semantics.

common/Smallstep.v
@@ -32,67 +32,64 @@ Set Implicit Arguments.
 
 Section CLOSURES.
 
-Variable genv: Type.
 Variable state: Type.
 
 (** A one-step transition relation has the following signature.
-  It is parameterized by a global environment, which does not
-  change during the transition.  It relates the initial state
-  of the transition with its final state.  The [trace] parameter
-  captures the observable events possibly generated during the
-  transition. *)
+  It relates the initial state of the transition with its final state.
+  The [trace] parameter captures the observable events possibly
+  generated during the transition. *)
 
-Variable step: genv -> state -> trace -> state -> Prop.
+Variable step: state -> trace -> state -> Prop.
 
 (** No transitions: stuck state *)
 
-Definition nostep (ge: genv) (s: state) : Prop :=
-  forall t s', ~(step ge s t s').
+Definition nostep (s: state) : Prop :=
+  forall t s', ~(step s t s').
 
 (** Zero, one or several transitions.  Also known as Kleene closure,
     or reflexive transitive closure. *)
 
-Inductive star (ge: genv): state -> trace -> state -> Prop :=
+Inductive star: state -> trace -> state -> Prop :=
   | star_refl: forall s,
-      star ge s E0 s
+      star s E0 s
   | star_step: forall s1 t1 s2 t2 s3 t,
-      step ge s1 t1 s2 -> star ge s2 t2 s3 -> t = t1 ** t2 ->
-      star ge s1 t s3.
+      step s1 t1 s2 -> star s2 t2 s3 -> t = t1 ** t2 ->
+      star s1 t s3.
 
 Lemma star_one:
-  forall ge s1 t s2, step ge s1 t s2 -> star ge s1 t s2.
+  forall s1 t s2, step s1 t s2 -> star s1 t s2.
 Proof.
   intros. eapply star_step; eauto. apply star_refl. traceEq.
 Qed.
 
 Lemma star_two:
-  forall ge s1 t1 s2 t2 s3 t,
-  step ge s1 t1 s2 -> step ge s2 t2 s3 -> t = t1 ** t2 ->
-  star ge s1 t s3.
+  forall s1 t1 s2 t2 s3 t,
+  step s1 t1 s2 -> step s2 t2 s3 -> t = t1 ** t2 ->
+  star s1 t s3.
 Proof.
   intros. eapply star_step; eauto. apply star_one; auto.
 Qed.
 
 Lemma star_three:
-  forall ge s1 t1 s2 t2 s3 t3 s4 t,
-  step ge s1 t1 s2 -> step ge s2 t2 s3 -> step ge s3 t3 s4 -> t = t1 ** t2 ** t3 ->
-  star ge s1 t s4.
+  forall s1 t1 s2 t2 s3 t3 s4 t,
+  step s1 t1 s2 -> step s2 t2 s3 -> step s3 t3 s4 -> t = t1 ** t2 ** t3 ->
+  star s1 t s4.
 Proof.
   intros. eapply star_step; eauto. eapply star_two; eauto.
 Qed.
 
 Lemma star_four:
-  forall ge s1 t1 s2 t2 s3 t3 s4 t4 s5 t,
-  step ge s1 t1 s2 -> step ge s2 t2 s3 ->
-  step ge s3 t3 s4 -> step ge s4 t4 s5 -> t = t1 ** t2 ** t3 ** t4 ->
-  star ge s1 t s5.
+  forall s1 t1 s2 t2 s3 t3 s4 t4 s5 t,
+  step s1 t1 s2 -> step s2 t2 s3 ->
+  step s3 t3 s4 -> step s4 t4 s5 -> t = t1 ** t2 ** t3 ** t4 ->
+  star s1 t s5.
 Proof.
   intros. eapply star_step; eauto. eapply star_three; eauto.
 Qed.
 
 Lemma star_trans:
-  forall ge s1 t1 s2, star ge s1 t1 s2 ->
-  forall t2 s3 t, star ge s2 t2 s3 -> t = t1 ** t2 -> star ge s1 t s3.
+  forall s1 t1 s2, star s1 t1 s2 ->
+  forall t2 s3 t, star s2 t2 s3 -> t = t1 ** t2 -> star s1 t s3.
 Proof.
   induction 1; intros.
   rewrite H0. simpl. auto.
@@ -100,27 +97,27 @@ Proof.
 Qed.
 
 Lemma star_left:
-  forall ge s1 t1 s2 t2 s3 t,
-  step ge s1 t1 s2 -> star ge s2 t2 s3 -> t = t1 ** t2 ->
-  star ge s1 t s3.
+  forall s1 t1 s2 t2 s3 t,
+  step s1 t1 s2 -> star s2 t2 s3 -> t = t1 ** t2 ->
+  star s1 t s3.
 Proof star_step.
 
 Lemma star_right:
-  forall ge s1 t1 s2 t2 s3 t,
-  star ge s1 t1 s2 -> step ge s2 t2 s3 -> t = t1 ** t2 ->
-  star ge s1 t s3.
+  forall s1 t1 s2 t2 s3 t,
+  star s1 t1 s2 -> step s2 t2 s3 -> t = t1 ** t2 ->
+  star s1 t s3.
 Proof.
   intros. eapply star_trans. eauto. apply star_one. eauto. auto.
 Qed.
 
 Lemma star_E0_ind:
-  forall ge (P: state -> state -> Prop),
+  forall (P: state -> state -> Prop),
   (forall s, P s s) ->
-  (forall s1 s2 s3, step ge s1 E0 s2 -> P s2 s3 -> P s1 s3) ->
-  forall s1 s2, star ge s1 E0 s2 -> P s1 s2.
+  (forall s1 s2 s3, step s1 E0 s2 -> P s2 s3 -> P s1 s3) ->
+  forall s1 s2, star s1 E0 s2 -> P s1 s2.
 Proof.
-  intros ge P BASE REC.
-  assert (forall s1 t s2, star ge s1 t s2 -> t = E0 -> P s1 s2).
+  intros P BASE REC.
+  assert (forall s1 t s2, star s1 t s2 -> t = E0 -> P s1 s2).
     induction 1; intros; subst.
     auto.
     destruct (Eapp_E0_inv _ _ H2). subst. eauto.
@@ -129,54 +126,54 @@ Qed.
 
 (** One or several transitions.  Also known as the transitive closure. *)
 
-Inductive plus (ge: genv): state -> trace -> state -> Prop :=
+Inductive plus: state -> trace -> state -> Prop :=
   | plus_left: forall s1 t1 s2 t2 s3 t,
-      step ge s1 t1 s2 -> star ge s2 t2 s3 -> t = t1 ** t2 ->
-      plus ge s1 t s3.
+      step s1 t1 s2 -> star s2 t2 s3 -> t = t1 ** t2 ->
+      plus s1 t s3.
 
 Lemma plus_one:
-  forall ge s1 t s2,
-  step ge s1 t s2 -> plus ge s1 t s2.
+  forall s1 t s2,
+  step s1 t s2 -> plus s1 t s2.
 Proof.
   intros. econstructor; eauto. apply star_refl. traceEq.
 Qed.
 
 Lemma plus_two:
-  forall ge s1 t1 s2 t2 s3 t,
-  step ge s1 t1 s2 -> step ge s2 t2 s3 -> t = t1 ** t2 ->
-  plus ge s1 t s3.
+  forall s1 t1 s2 t2 s3 t,
+  step s1 t1 s2 -> step s2 t2 s3 -> t = t1 ** t2 ->
+  plus s1 t s3.
 Proof.
   intros. eapply plus_left; eauto. apply star_one; auto.
 Qed.
 
 Lemma plus_three:
-  forall ge s1 t1 s2 t2 s3 t3 s4 t,
-  step ge s1 t1 s2 -> step ge s2 t2 s3 -> step ge s3 t3 s4 -> t = t1 ** t2 ** t3 ->
-  plus ge s1 t s4.
+  forall s1 t1 s2 t2 s3 t3 s4 t,
+  step s1 t1 s2 -> step s2 t2 s3 -> step s3 t3 s4 -> t = t1 ** t2 ** t3 ->
+  plus s1 t s4.
 Proof.
   intros. eapply plus_left; eauto. eapply star_two; eauto.
 Qed.
 
 Lemma plus_four:
-  forall ge s1 t1 s2 t2 s3 t3 s4 t4 s5 t,
-  step ge s1 t1 s2 -> step ge s2 t2 s3 ->
-  step ge s3 t3 s4 -> step ge s4 t4 s5 -> t = t1 ** t2 ** t3 ** t4 ->
-  plus ge s1 t s5.
+  forall s1 t1 s2 t2 s3 t3 s4 t4 s5 t,
+  step s1 t1 s2 -> step s2 t2 s3 ->
+  step s3 t3 s4 -> step s4 t4 s5 -> t = t1 ** t2 ** t3 ** t4 ->
+  plus s1 t s5.
 Proof.
   intros. eapply plus_left; eauto. eapply star_three; eauto.
 Qed.
 
 Lemma plus_star:
-  forall ge s1 t s2, plus ge s1 t s2 -> star ge s1 t s2.
+  forall s1 t s2, plus s1 t s2 -> star s1 t s2.
 Proof.
   intros. inversion H; subst.
   eapply star_step; eauto.
 Qed.
 
 Lemma plus_right:
-  forall ge s1 t1 s2 t2 s3 t,
-  star ge s1 t1 s2 -> step ge s2 t2 s3 -> t = t1 ** t2 ->
-  plus ge s1 t s3.
+  forall s1 t1 s2 t2 s3 t,
+  star s1 t1 s2 -> step s2 t2 s3 -> t = t1 ** t2 ->
+  plus s1 t s3.
 Proof.
   intros. inversion H; subst. simpl. apply plus_one. auto.
   rewrite Eapp_assoc. eapply plus_left; eauto.
@@ -184,24 +181,24 @@ Proof.
 Qed.
 
 Lemma plus_left':
-  forall ge s1 t1 s2 t2 s3 t,
-  step ge s1 t1 s2 -> plus ge s2 t2 s3 -> t = t1 ** t2 ->
-  plus ge s1 t s3.
+  forall s1 t1 s2 t2 s3 t,
+  step s1 t1 s2 -> plus s2 t2 s3 -> t = t1 ** t2 ->
+  plus s1 t s3.
 Proof.
   intros. eapply plus_left; eauto. apply plus_star; auto.
 Qed.
 
 Lemma plus_right':
-  forall ge s1 t1 s2 t2 s3 t,
-  plus ge s1 t1 s2 -> step ge s2 t2 s3 -> t = t1 ** t2 ->
-  plus ge s1 t s3.
+  forall s1 t1 s2 t2 s3 t,
+  plus s1 t1 s2 -> step s2 t2 s3 -> t = t1 ** t2 ->
+  plus s1 t s3.
 Proof.
   intros. eapply plus_right; eauto. apply plus_star; auto.
 Qed.
 
 Lemma plus_star_trans:
-  forall ge s1 t1 s2 t2 s3 t,
-  plus ge s1 t1 s2 -> star ge s2 t2 s3 -> t = t1 ** t2 -> plus ge s1 t s3.
+  forall s1 t1 s2 t2 s3 t,
+  plus s1 t1 s2 -> star s2 t2 s3 -> t = t1 ** t2 -> plus s1 t s3.
 Proof.
   intros. inversion H; subst.
   econstructor; eauto. eapply star_trans; eauto.
@@ -209,8 +206,8 @@ Proof.
 Qed.
 
 Lemma star_plus_trans:
-  forall ge s1 t1 s2 t2 s3 t,
-  star ge s1 t1 s2 -> plus ge s2 t2 s3 -> t = t1 ** t2 -> plus ge s1 t s3.
+  forall s1 t1 s2 t2 s3 t,
+  star s1 t1 s2 -> plus s2 t2 s3 -> t = t1 ** t2 -> plus s1 t s3.
 Proof.
   intros. inversion H; subst.
   simpl; auto.
@@ -220,16 +217,16 @@ Proof.
 Qed.
 
 Lemma plus_trans:
-  forall ge s1 t1 s2 t2 s3 t,
-  plus ge s1 t1 s2 -> plus ge s2 t2 s3 -> t = t1 ** t2 -> plus ge s1 t s3.
+  forall s1 t1 s2 t2 s3 t,
+  plus s1 t1 s2 -> plus s2 t2 s3 -> t = t1 ** t2 -> plus s1 t s3.
 Proof.
   intros. eapply plus_star_trans. eauto. apply plus_star. eauto. auto.
 Qed.
 
 Lemma plus_inv:
-  forall ge s1 t s2,
-  plus ge s1 t s2 ->
-  step ge s1 t s2 \/ exists s', exists t1, exists t2, step ge s1 t1 s' /\ plus ge s' t2 s2 /\ t = t1 ** t2.
+  forall s1 t s2,
+  plus s1 t s2 ->
+  step s1 t s2 \/ exists s', exists t1, exists t2, step s1 t1 s' /\ plus s' t2 s2 /\ t = t1 ** t2.
 Proof.
   intros. inversion H; subst. inversion H1; subst.
   left. rewrite E0_right. auto.
@@ -238,24 +235,24 @@ Proof.
 Qed.
 
 Lemma star_inv:
-  forall ge s1 t s2,
-  star ge s1 t s2 ->
-  (s2 = s1 /\ t = E0) \/ plus ge s1 t s2.
+  forall s1 t s2,
+  star s1 t s2 ->
+  (s2 = s1 /\ t = E0) \/ plus s1 t s2.
 Proof.
   intros. inv H. left; auto. right; econstructor; eauto.
 Qed.
 
 Lemma plus_ind2:
-  forall ge (P: state -> trace -> state -> Prop),
-  (forall s1 t s2, step ge s1 t s2 -> P s1 t s2) ->
+  forall (P: state -> trace -> state -> Prop),
+  (forall s1 t s2, step s1 t s2 -> P s1 t s2) ->
   (forall s1 t1 s2 t2 s3 t,
-   step ge s1 t1 s2 -> plus ge s2 t2 s3 -> P s2 t2 s3 -> t = t1 ** t2 ->
+   step s1 t1 s2 -> plus s2 t2 s3 -> P s2 t2 s3 -> t = t1 ** t2 ->
    P s1 t s3) ->
-  forall s1 t s2, plus ge s1 t s2 -> P s1 t s2.
+  forall s1 t s2, plus s1 t s2 -> P s1 t s2.
 Proof.
-  intros ge P BASE IND.
-  assert (forall s1 t s2, star ge s1 t s2 ->
-         forall s0 t0, step ge s0 t0 s1 ->
+  intros P BASE IND.
+  assert (forall s1 t s2, star s1 t s2 ->
+         forall s0 t0, step s0 t0 s1 ->
          P s0 (t0 ** t) s2).
   induction 1; intros.
   rewrite E0_right. apply BASE; auto.
@@ -265,30 +262,30 @@ Proof.
 Qed.
 
 Lemma plus_E0_ind:
-  forall ge (P: state -> state -> Prop),
-  (forall s1 s2 s3, step ge s1 E0 s2 -> star ge s2 E0 s3 -> P s1 s3) ->
-  forall s1 s2, plus ge s1 E0 s2 -> P s1 s2.
+  forall (P: state -> state -> Prop),
+  (forall s1 s2 s3, step s1 E0 s2 -> star s2 E0 s3 -> P s1 s3) ->
+  forall s1 s2, plus s1 E0 s2 -> P s1 s2.
 Proof.
   intros. inv H0. exploit Eapp_E0_inv; eauto. intros [A B]; subst. eauto.
 Qed.
 
 (** Counted sequences of transitions *)
 
-Inductive starN (ge: genv): nat -> state -> trace -> state -> Prop :=
+Inductive starN: nat -> state -> trace -> state -> Prop :=
   | starN_refl: forall s,
-      starN ge O s E0 s
+      starN O s E0 s
   | starN_step: forall n s t t1 s' t2 s'',
-      step ge s t1 s' -> starN ge n s' t2 s'' -> t = t1 ** t2 ->
-      starN ge (S n) s t s''.
+      step s t1 s' -> starN n s' t2 s'' -> t = t1 ** t2 ->
+      starN (S n) s t s''.
 
 Remark starN_star:
-  forall ge n s t s', starN ge n s t s' -> star ge s t s'.
+  forall n s t s', starN n s t s' -> star s t s'.
 Proof.
   induction 1; econstructor; eauto.
 Qed.
 
 Remark star_starN:
-  forall ge s t s', star ge s t s' -> exists n, starN ge n s t s'.
+  forall s t s', star s t s' -> exists n, starN n s t s'.
 Proof.
   induction 1.
   exists O; constructor.
@@ -297,15 +294,15 @@ Qed.
 
 (** Infinitely many transitions *)
 
-CoInductive forever (ge: genv): state -> traceinf -> Prop :=
+CoInductive forever: state -> traceinf -> Prop :=
   | forever_intro: forall s1 t s2 T,
-      step ge s1 t s2 -> forever ge s2 T ->
-      forever ge s1 (t *** T).
+      step s1 t s2 -> forever s2 T ->
+      forever s1 (t *** T).
 
 Lemma star_forever:
-  forall ge s1 t s2, star ge s1 t s2 ->
-  forall T, forever ge s2 T ->
-  forever ge s1 (t *** T).
+  forall s1 t s2, star s1 t s2 ->
+  forall T, forever s2 T ->
+  forever s1 (t *** T).
 Proof.
   induction 1; intros. simpl. auto.
   subst t. rewrite Eappinf_assoc.
@@ -318,28 +315,28 @@ Qed.
 Variable A: Type.
 Variable order: A -> A -> Prop.
 
-CoInductive forever_N (ge: genv) : A -> state -> traceinf -> Prop :=
+CoInductive forever_N: A -> state -> traceinf -> Prop :=
   | forever_N_star: forall s1 t s2 a1 a2 T1 T2,
-      star ge s1 t s2 ->
+      star s1 t s2 ->
       order a2 a1 ->
-      forever_N ge a2 s2 T2 ->
+      forever_N a2 s2 T2 ->
       T1 = t *** T2 ->
-      forever_N ge a1 s1 T1
+      forever_N a1 s1 T1
   | forever_N_plus: forall s1 t s2 a1 a2 T1 T2,
-      plus ge s1 t s2 ->
-      forever_N ge a2 s2 T2 ->
+      plus s1 t s2 ->
+      forever_N a2 s2 T2 ->
       T1 = t *** T2 ->
-      forever_N ge a1 s1 T1.
+      forever_N a1 s1 T1.
 
 Hypothesis order_wf: well_founded order.
 
 Lemma forever_N_inv:
-  forall ge a s T,
-  forever_N ge a s T ->
+  forall a s T,
+  forever_N a s T ->
   exists t, exists s', exists a', exists T',
-  step ge s t s' /\ forever_N ge a' s' T' /\ T = t *** T'.
+  step s t s' /\ forever_N a' s' T' /\ T = t *** T'.
 Proof.
-  intros ge a0. pattern a0. apply (well_founded_ind order_wf).
+  intros a0. pattern a0. apply (well_founded_ind order_wf).
   intros. inv H0.
   (* star case *)
   inv H1.
@@ -359,7 +356,7 @@ Proof.
 Qed.
 
 Lemma forever_N_forever:
-  forall ge a s T, forever_N ge a s T -> forever ge s T.
+  forall a s T, forever_N a s T -> forever s T.
 Proof.
   cofix COINDHYP; intros.
   destruct (forever_N_inv H) as [t [s' [a' [T' [P [Q R]]]]]].
@@ -369,18 +366,18 @@ Qed.
 
 (** Yet another alternative definition of [forever]. *)
 
-CoInductive forever_plus (ge: genv) : state -> traceinf -> Prop :=
+CoInductive forever_plus: state -> traceinf -> Prop :=
   | forever_plus_intro: forall s1 t s2 T1 T2,
-      plus ge s1 t s2 ->
-      forever_plus ge s2 T2 ->
+      plus s1 t s2 ->
+      forever_plus s2 T2 ->
       T1 = t *** T2 ->
-      forever_plus ge s1 T1.
+      forever_plus s1 T1.
 
 Lemma forever_plus_inv:
-  forall ge s T,
-  forever_plus ge s T ->
+  forall s T,
+  forever_plus s T ->
   exists s', exists t, exists T',
-  step ge s t s' /\ forever_plus ge s' T' /\ T = t *** T'.
+  step s t s' /\ forever_plus s' T' /\ T = t *** T'.
 Proof.
   intros. inv H. inv H0. exists s0; exists t1; exists (t2 *** T2).
   split. auto.
@@ -390,7 +387,7 @@ Proof.
 Qed.
 
 Lemma forever_plus_forever:
-  forall ge s T, forever_plus ge s T -> forever ge s T.
+  forall s T, forever_plus s T -> forever s T.
 Proof.
   cofix COINDHYP; intros.
   destruct (forever_plus_inv H) as [s' [t [T' [P [Q R]]]]].
@@ -399,31 +396,31 @@ Qed.
 
 (** Infinitely many silent transitions *)
 
-CoInductive forever_silent (ge: genv): state -> Prop :=
+CoInductive forever_silent: state -> Prop :=
   | forever_silent_intro: forall s1 s2,
-      step ge s1 E0 s2 -> forever_silent ge s2 ->
-      forever_silent ge s1.
+      step s1 E0 s2 -> forever_silent s2 ->
+      forever_silent s1.
 
 (** An alternate definition. *)
 
-CoInductive forever_silent_N (ge: genv) : A -> state -> Prop :=
+CoInductive forever_silent_N: A -> state -> Prop :=
   | forever_silent_N_star: forall s1 s2 a1 a2,
-      star ge s1 E0 s2 ->
+      star s1 E0 s2 ->
       order a2 a1 ->
-      forever_silent_N ge a2 s2 ->
-      forever_silent_N ge a1 s1
+      forever_silent_N a2 s2 ->
+      forever_silent_N a1 s1
   | forever_silent_N_plus: forall s1 s2 a1 a2,
-      plus ge s1 E0 s2 ->
-      forever_silent_N ge a2 s2 ->
-      forever_silent_N ge a1 s1.
+      plus s1 E0 s2 ->
+      forever_silent_N a2 s2 ->
+      forever_silent_N a1 s1.
 
 Lemma forever_silent_N_inv:
-  forall ge a s,
-  forever_silent_N ge a s ->
+  forall a s,
+  forever_silent_N a s ->
   exists s', exists a',
-  step ge s E0 s' /\ forever_silent_N ge a' s'.
+  step s E0 s' /\ forever_silent_N a' s'.
 Proof.
-  intros ge a0. pattern a0. apply (well_founded_ind order_wf).
+  intros a0. pattern a0. apply (well_founded_ind order_wf).
   intros. inv H0.
   (* star case *)
   inv H1.
@@ -441,7 +438,7 @@ Proof.
 Qed.
 
 Lemma forever_silent_N_forever:
-  forall ge a s, forever_silent_N ge a s -> forever_silent ge s.
+  forall a s, forever_silent_N a s -> forever_silent s.
 Proof.
   cofix COINDHYP; intros.
   destruct (forever_silent_N_inv H) as [s' [a' [P Q]]].
@@ -451,15 +448,15 @@ Qed.
 
 (** Infinitely many non-silent transitions *)
 
-CoInductive forever_reactive (ge: genv): state -> traceinf -> Prop :=
+CoInductive forever_reactive: state -> traceinf -> Prop :=
   | forever_reactive_intro: forall s1 s2 t T,
-      star ge s1 t s2 -> t <> E0 -> forever_reactive ge s2 T ->
-      forever_reactive ge s1 (t *** T).
+      star s1 t s2 -> t <> E0 -> forever_reactive s2 T ->
+      forever_reactive s1 (t *** T).
 
 Lemma star_forever_reactive:
-  forall ge s1 t s2 T,
-  star ge s1 t s2 -> forever_reactive ge s2 T ->
-  forever_reactive ge s1 (t *** T).
+  forall s1 t s2 T,
+  star s1 t s2 -> forever_reactive s2 T ->
+  forever_reactive s1 (t *** T).
 Proof.
   intros. inv H0. rewrite <- Eappinf_assoc. econstructor.
   eapply star_trans; eauto.
@@ -475,11 +472,9 @@ End CLOSURES.
 
 Record semantics : Type := Semantics_gen {
   state: Type;
-  genvtype: Type;
-  step : genvtype -> state -> trace -> state -> Prop;
+  step : state -> trace -> state -> Prop;
   initial_state: state -> Prop;
   final_state: state -> int -> Prop;
-  globalenv: genvtype;
   symbolenv: Senv.t
 }.
 
@@ -491,21 +486,19 @@ Definition Semantics {state funtype vartype: Type}
                      (final_state: state -> int -> Prop)
                      (globalenv: Genv.t funtype vartype) :=
   {| state := state;
-     genvtype := Genv.t funtype vartype;
-     step := step;
+     step := step globalenv;
      initial_state := initial_state;
      final_state := final_state;
-     globalenv := globalenv;
      symbolenv := Genv.to_senv globalenv |}.
 
 (** Handy notations. *)
 
-Notation " 'Step' L " := (step L (globalenv L)) (at level 1) : smallstep_scope.
-Notation " 'Star' L " := (star (step L) (globalenv L)) (at level 1) : smallstep_scope.
-Notation " 'Plus' L " := (plus (step L) (globalenv L)) (at level 1) : smallstep_scope.
-Notation " 'Forever_silent' L " := (forever_silent (step L) (globalenv L)) (at level 1) : smallstep_scope.
-Notation " 'Forever_reactive' L " := (forever_reactive (step L) (globalenv L)) (at level 1) : smallstep_scope.
-Notation " 'Nostep' L " := (nostep (step L) (globalenv L)) (at level 1) : smallstep_scope.
+Notation " 'Step' L " := (step L) (at level 1) : smallstep_scope.
+Notation " 'Star' L " := (star (step L)) (at level 1) : smallstep_scope.
+Notation " 'Plus' L " := (plus (step L)) (at level 1) : smallstep_scope.
+Notation " 'Forever_silent' L " := (forever_silent (step L)) (at level 1) : smallstep_scope.
+Notation " 'Forever_reactive' L " := (forever_reactive (step L)) (at level 1) : smallstep_scope.
+Notation " 'Nostep' L " := (nostep (step L)) (at level 1) : smallstep_scope.
 
 Open Scope smallstep_scope.
 
@@ -759,7 +752,7 @@ Lemma simulation_forever_silent:
 Proof.
   assert (forall i s1 s2,
           Forever_silent L1 s1 -> match_states i s1 s2 ->
-          forever_silent_N (step L2) order (globalenv L2) i s2).
+          forever_silent_N (step L2) order i s2).
     cofix COINDHYP; intros.
     inv H. destruct (fsim_simulation S _ _ _ H1 _ _ H0) as [i' [s2' [A B]]].
     destruct A as [C | [C D]].
@@ -1374,17 +1367,17 @@ Inductive f2b_match_states: f2b_index -> state L1 -> state L2 -> Prop :=
   | f2b_match_before: forall s1 t s1' s2b s2 n s2a i,
       Step L1 s1 t s1' ->  t <> E0 ->
       Star L2 s2b E0 s2 ->
-      starN (step L2) (globalenv L2) n s2 t s2a ->
+      starN (step L2) n s2 t s2a ->
       match_states i s1 s2b ->
       f2b_match_states (F2BI_before n) s1 s2
   | f2b_match_after: forall n s2 s2a s1 i,
-      starN (step L2) (globalenv L2) (S n) s2 E0 s2a ->
+      starN (step L2) (S n) s2 E0 s2a ->
       match_states i s1 s2a ->
       f2b_match_states (F2BI_after (S n)) s1 s2.
 
 Remark f2b_match_after':
   forall n s2 s2a s1 i,
-  starN (step L2) (globalenv L2) n s2 E0 s2a ->
+  starN (step L2) n s2 E0 s2a ->
   match_states i s1 s2a ->
   f2b_match_states (F2BI_after n) s1 s2.
 Proof.
@@ -1536,24 +1529,22 @@ Variable L: semantics.
 
 Hypothesis Lwb: well_behaved_traces L.
 
-Inductive atomic_step (ge: genvtype L): (trace * state L) -> trace -> (trace * state L) -> Prop :=
+Inductive atomic_step: (trace * state L) -> trace -> (trace * state L) -> Prop :=
   | atomic_step_silent: forall s s',
       Step L s E0 s' ->
-      atomic_step ge (E0, s) E0 (E0, s')
+      atomic_step (E0, s) E0 (E0, s')
   | atomic_step_start: forall s ev t s',
       Step L s (ev :: t) s' ->
-      atomic_step ge (E0, s) (ev :: nil) (t, s')
+      atomic_step (E0, s) (ev :: nil) (t, s')
   | atomic_step_continue: forall ev t s,
       output_trace (ev :: t) ->
-      atomic_step ge (ev :: t, s) (ev :: nil) (t, s).
+      atomic_step (ev :: t, s) (ev :: nil) (t, s).
 
 Definition atomic : semantics := {|
   state := (trace * state L)%type;
-  genvtype := genvtype L;
   step := atomic_step;
   initial_state := fun s => initial_state L (snd s) /\ fst s = E0;
   final_state := fun s r => final_state L (snd s) r /\ fst s = E0;
-  globalenv := globalenv L;
   symbolenv := symbolenv L
 |}.
 
@@ -1806,6 +1797,6 @@ Record bigstep_sound (B: bigstep_semantics) (L: semantics) : Prop :=
     bigstep_diverges_sound:
       forall T,
       bigstep_diverges B T ->
-      exists s1, initial_state L s1 /\ forever (step L) (globalenv L) s1 T
+      exists s1, initial_state L s1 /\ forever (step L) s1 T
 }.
 
