backend/Inliningproof.v
@@ -224,8 +224,8 @@ Lemma tr_moves_init_regs:
   (forall r, In r rdsts -> Ple r ctx2.(mreg)) ->
   list_forall2 (val_reg_charact F ctx1 rs1) vl rsrcs ->
   exists rs2,
-    star step tge (State stk f sp pc1 rs1 m)
-               E0 (State stk f sp pc2 rs2 m)
+    star (step tge) (State stk f sp pc1 rs1 m)
+                 E0 (State stk f sp pc2 rs2 m)
   /\ agree_regs F ctx2 (init_regs vl rdsts) rs2
   /\ forall r, Plt r ctx2.(dreg) -> rs2#r = rs1#r.
 Proof.
@@ -933,7 +933,7 @@ Theorem step_simulation:
   forall S1 t S2,
   step ge S1 t S2 ->
   forall S1' (MS: match_states S1 S1'),
-  (exists S2', plus step tge S1' t S2' /\ match_states S2 S2')
+  (exists S2', plus (step tge) S1' t S2' /\ match_states S2 S2')
   \/ (measure S2 < measure S1 /\ t = E0 /\ match_states S2 S1')%nat.
 Proof.
   induction 1; intros; inv MS.
