backend/Linearizeproof.v
@@ -252,8 +252,8 @@ Lemma starts_with_correct:
   unique_labels c2 ->
   starts_with lbl c1 = true ->
   find_label lbl c2 = Some c3 ->
-  plus step tge (State s f sp c1 ls m)
-             E0 (State s f sp c3 ls m).
+  plus (step tge) (State s f sp c1 ls m)
+               E0 (State s f sp c3 ls m).
 Proof.
   induction c1.
   simpl; intros; discriminate.
@@ -456,8 +456,8 @@ Lemma add_branch_correct:
   transf_function f = OK tf ->
   is_tail k tf.(fn_code) ->
   find_label lbl tf.(fn_code) = Some c ->
-  plus step tge (State s tf sp (add_branch lbl k) ls m)
-             E0 (State s tf sp c ls m).
+  plus (step tge) (State s tf sp (add_branch lbl k) ls m)
+               E0 (State s tf sp c ls m).
 Proof.
   intros. unfold add_branch.
   caseEq (starts_with lbl k); intro SW.
@@ -556,7 +556,7 @@ Qed.
 Theorem transf_step_correct:
   forall s1 t s2, LTL.step ge s1 t s2 ->
   forall s1' (MS: match_states s1 s1'),
-  (exists s2', plus Linear.step tge s1' t s2' /\ match_states s2 s2')
+  (exists s2', plus (Linear.step tge) s1' t s2' /\ match_states s2 s2')
   \/ (measure s2 < measure s1 /\ t = E0 /\ match_states s2 s1')%nat.
 Proof.
   induction 1; intros; try (inv MS).
