backend/Stackingproof.v
@@ -909,7 +909,7 @@ Lemma save_callee_save_rec_correct:
   m |= range sp pos (size_callee_save_area_rec l pos) ** P ->
   agree_regs j ls rs ->
   exists rs', exists m',
-     star step tge
+     star (step tge)
         (State cs fb (Vptr sp Ptrofs.zero) (save_callee_save_rec l pos k) rs m)
      E0 (State cs fb (Vptr sp Ptrofs.zero) k rs' m')
   /\ m' |= contains_callee_saves j sp pos l ls ** P
@@ -1000,9 +1000,9 @@ Lemma save_callee_save_correct:
   let ls1 := LTL.undef_regs destroyed_at_function_entry (LTL.call_regs ls) in
   let rs1 := undef_regs destroyed_at_function_entry rs in
   exists rs', exists m',
-     star step tge
-        (State cs fb (Vptr sp Ptrofs.zero) (save_callee_save fe k) rs1 m)
-     E0 (State cs fb (Vptr sp Ptrofs.zero) k rs' m')
+     star (step tge)
+          (State cs fb (Vptr sp Ptrofs.zero) (save_callee_save fe k) rs1 m)
+       E0 (State cs fb (Vptr sp Ptrofs.zero) k rs' m')
   /\ m' |= contains_callee_saves j sp fe.(fe_ofs_callee_save) b.(used_callee_save) ls0 ** P
   /\ (forall ofs k p, Mem.perm m sp ofs k p -> Mem.perm m' sp ofs k p)
   /\ agree_regs j ls1 rs'.
@@ -1050,9 +1050,9 @@ Lemma function_prologue_correct:
      Mem.alloc m1' 0 tf.(fn_stacksize) = (m2', sp')
   /\ store_stack m2' (Vptr sp' Ptrofs.zero) Tptr tf.(fn_link_ofs) parent = Some m3'
   /\ store_stack m3' (Vptr sp' Ptrofs.zero) Tptr tf.(fn_retaddr_ofs) ra = Some m4'
-  /\ star step tge
-         (State cs fb (Vptr sp' Ptrofs.zero) (save_callee_save fe k) rs1 m4')
-      E0 (State cs fb (Vptr sp' Ptrofs.zero) k rs' m5')
+  /\ star (step tge)
+          (State cs fb (Vptr sp' Ptrofs.zero) (save_callee_save fe k) rs1 m4')
+       E0 (State cs fb (Vptr sp' Ptrofs.zero) k rs' m5')
   /\ agree_regs j' ls1 rs'
   /\ agree_locs ls1 ls0
   /\ m5' |= frame_contents j' sp' ls1 ls0 parent ra ** minjection j' m2 ** globalenv_inject ge j' ** P
@@ -1171,7 +1171,7 @@ Lemma restore_callee_save_rec_correct:
   agree_unused ls0 rs ->
   (forall r, In r l -> mreg_within_bounds b r) ->
   exists rs',
-    star step tge
+    star (step tge)
       (State cs fb (Vptr sp Ptrofs.zero) (restore_callee_save_rec l ofs k) rs m)
    E0 (State cs fb (Vptr sp Ptrofs.zero) k rs' m)
   /\ (forall r, In r l -> Val.inject j (ls0 (R r)) (rs' r))
@@ -1216,7 +1216,7 @@ Lemma restore_callee_save_correct:
   m |= frame_contents j sp ls ls0 pa ra ** P ->
   agree_unused j ls0 rs ->
   exists rs',
-    star step tge
+    star (step tge)
        (State cs fb (Vptr sp Ptrofs.zero) (restore_callee_save fe k) rs m)
     E0 (State cs fb (Vptr sp Ptrofs.zero) k rs' m)
   /\ (forall r,
@@ -1255,7 +1255,7 @@ Lemma function_epilogue_correct:
      load_stack m' (Vptr sp' Ptrofs.zero) Tptr tf.(fn_link_ofs) = Some pa
   /\ load_stack m' (Vptr sp' Ptrofs.zero) Tptr tf.(fn_retaddr_ofs) = Some ra
   /\ Mem.free m' sp' 0 tf.(fn_stacksize) = Some m1'
-  /\ star step tge
+  /\ star (step tge)
        (State cs fb (Vptr sp' Ptrofs.zero) (restore_callee_save fe k) rs m')
     E0 (State cs fb (Vptr sp' Ptrofs.zero) k rs1 m')
   /\ agree_regs j (return_regs ls0 ls) rs1
@@ -1804,7 +1804,7 @@ Inductive match_states: Linear.state -> Mach.state -> Prop :=
 Theorem transf_step_correct:
   forall s1 t s2, Linear.step ge s1 t s2 ->
   forall (WTS: wt_state s1) s1' (MS: match_states s1 s1'),
-  exists s2', plus step tge s1' t s2' /\ match_states s2 s2'.
+  exists s2', plus (step tge) s1' t s2' /\ match_states s2 s2'.
 Proof.
   induction 1; intros;
   try inv MS;
