cfrontend/ClightBigstep.v
@@ -300,14 +300,14 @@ Lemma exec_stmt_eval_funcall_steps:
   (forall e le m s t le' m' out,
    exec_stmt ge e le m s t le' m' out ->
    forall f k, exists S,
-   star step1 ge (State f s k e le m) t S
+   star (step1 ge) (State f s k e le m) t S
    /\ outcome_state_match e le' m' f k out S)
 /\
   (forall m fd args t m' res,
    eval_funcall ge m fd args t m' res ->
    forall k,
    is_call_cont k ->
-   star step1 ge (Callstate fd args k m) t (Returnstate res k m')).
+   star (step1 ge) (Callstate fd args k m) t (Returnstate res k m')).
 Proof.
   apply exec_stmt_funcall_ind; intros.
 
@@ -478,7 +478,7 @@ Lemma exec_stmt_steps:
    forall e le m s t le' m' out,
    exec_stmt ge e le m s t le' m' out ->
    forall f k, exists S,
-   star step1 ge (State f s k e le m) t S
+   star (step1 ge) (State f s k e le m) t S
    /\ outcome_state_match e le' m' f k out S.
 Proof (proj1 exec_stmt_eval_funcall_steps).
 
@@ -487,7 +487,7 @@ Lemma eval_funcall_steps:
    eval_funcall ge m fd args t m' res ->
    forall k,
    is_call_cont k ->
-   star step1 ge (Callstate fd args k m) t (Returnstate res k m').
+   star (step1 ge) (Callstate fd args k m) t (Returnstate res k m').
 Proof (proj2 exec_stmt_eval_funcall_steps).
 
 Definition order (x y: unit) := False.
@@ -495,12 +495,12 @@ Definition order (x y: unit) := False.
 Lemma evalinf_funcall_forever:
   forall m fd args T k,
   evalinf_funcall ge m fd args T ->
-  forever_N step1 order ge tt (Callstate fd args k m) T.
+  forever_N (step1 ge) order tt (Callstate fd args k m) T.
 Proof.
   cofix CIH_FUN.
   assert (forall e le m s T f k,
           execinf_stmt ge e le m s T ->
-          forever_N step1 order ge tt (State f s k e le m) T).
+          forever_N (step1 ge) order tt (State f s k e le m) T).
   cofix CIH_STMT.
   intros. inv H.
 
